Add a lot of ReturnCall cases all over
Wish I'd split up this commit a bit more.

WebAssembly/Wasm.thy
@@ -201,7 +201,8 @@ inductive reduce :: "[s, v list, e list, nat, s, v list, e list] \<Rightarrow> b
 | call_indirect_Some:"\<lbrakk>stab s i (nat_of_int c) = Some cl; stypes s i j = tf; cl_type cl = tf\<rbrakk> \<Longrightarrow> \<lparr>s;vs;[$C (ConstInt32 c), $(Call_indirect j)]\<rparr> \<leadsto>_i \<lparr>s;vs;[Callcl cl]\<rparr>"
 | call_indirect_None:"\<lbrakk>(stab s i (nat_of_int c) = Some cl \<and> stypes s i j \<noteq> cl_type cl) \<or> stab s i (nat_of_int c) = None\<rbrakk> \<Longrightarrow> \<lparr>s;vs;[$C (ConstInt32 c), $(Call_indirect j)]\<rparr> \<leadsto>_i \<lparr>s;vs;[Trap]\<rparr>"
   \<comment> \<open>\<open>return_call\<close>\<close>
-| return_call: "\<lbrakk>const_list vs'; length vs' = n; Lfilled j lholed (vs' @ [$ReturnCall j']) es\<rbrakk>  \<Longrightarrow> \<lparr>s;vs;[Local n i' vls es]\<rparr> \<leadsto>_i \<lparr>s;vs;vs'@[Callcl (sfunc s i j')]\<rparr>"
+(* FIXME *)
+| return_call: "\<lbrakk>const_list vs'; length vs' = n; Lfilled j lholed (vs' @ [$ReturnCall j']) es\<rbrakk>  \<Longrightarrow> \<lparr>s;vs;[Local n i' vls es]\<rparr> \<leadsto>_i \<lparr>s;vs;[Callcl (sfunc s i j')]\<rparr>"
   \<comment> \<open>\<open>call_indirect\<close>\<close>
 | return_call_indirect_Some:"\<lbrakk>stab s i (nat_of_int c) = Some cl; stypes s i j = tf; cl_type cl = tf\<rbrakk> \<Longrightarrow> \<lparr>s;vs;[$C (ConstInt32 c), $(ReturnCall_indirect j)]\<rparr> \<leadsto>_i \<lparr>s;vs;[$(ReturnCall (nat_of_int c))]\<rparr>"
 | return_call_indirect_None:"\<lbrakk>(stab s i (nat_of_int c) = Some cl \<and> stypes s i j \<noteq> cl_type cl) \<or> stab s i (nat_of_int c) = None\<rbrakk> \<Longrightarrow> \<lparr>s;vs;[$C (ConstInt32 c), $(ReturnCall_indirect j)]\<rparr> \<leadsto>_i \<lparr>s;vs;[Trap]\<rparr>"
